<<<<<<< HEAD
@prefix dash: <http://datashapes.org/dash#> .
@prefix rdf: <http://www.w3.org/1999/02/22-rdf-syntax-ns#> .
@prefix rdfs: <http://www.w3.org/2000/01/rdf-schema#> .
@prefix schema: <http://schema.org/> .
@prefix sh: <http://www.w3.org/ns/shacl#> .
@prefix xsd: <http://www.w3.org/2001/XMLSchema#> .
@prefix owl: <http://www.w3.org/2002/07/owl#> .
@prefix skos: <http://www.w3.org/2004/02/skos/core#> .
@prefix :   <https://w3id.org/EnergyInformationModel/profiles/ontologyprofile/ontologyshape#> .



################################################################
####  sh:NodeShapes
###############################################################

:ClassShape
    a sh:NodeShape ;
    sh:targetClass owl:Class ;
    sh:property :PrefLabelShape ;
    sh:property :DefinitionShape .
    
:ObjectPropertyShape
    a sh:NodeShape ;
    sh:targetClass owl:ObjectProperty ;
    sh:property :PrefLabelShape ;
    sh:property :DefinitionShape ;
    sh:property :DomainShape ;
    sh:property [
        rdfs:comment "At least one range is defined to ensure correct transformation to OO artifacts"@en;
        sh:path rdfs:range ;
        sh:node :ClassShape ;
        sh:minCount 1 ;
    ] .



:DatatypePropertyShape
    a sh:NodeShape ;
    sh:targetClass owl:DatatypeProperty ;
    sh:property :PrefLabelShape ;
    sh:property :DefinitionShape ;
    sh:property [
        rdfs:comment "At least one range is defined to ensure correct transformation to OO artifacts"@en;
        sh:path rdfs:range ;
        sh:minCount 1 ;
    ] .


################################################################
####  sh:PropertyShapes
###############################################################


:PrefLabelShape 
    a sh:PropertyShape   ;
    rdfs:comment "Any class has at most one prefLabel for each language, each class has at least one prefLabel in one language"@en;
    sh:path skos:prefLabel ;
    sh:datatype xsd:string ;
    sh:minCount 1 .

:DefinitionShape 
    a sh:PropertyShape ;
    rdfs:comment "Any resource has at least one definition in one language"@en ;
    sh:path skos:definition ;
    sh:datatype xsd:string ;
    sh:minCount 1 .

:DomainShape 
    a sh:PropertyShape ;
    rdfs:comment "At least one domain is defined to ensure correct transformation to OO artifacts"@en;
    sh:path rdfs:domain ;
    sh:node :ClassShape ;
    sh:minCount 1 .
=======
@prefix dash: <http://datashapes.org/dash#> .
@prefix rdf: <http://www.w3.org/1999/02/22-rdf-syntax-ns#> .
@prefix rdfs: <http://www.w3.org/2000/01/rdf-schema#> .
@prefix schema: <http://schema.org/> .
@prefix sh: <http://www.w3.org/ns/shacl#> .
@prefix xsd: <http://www.w3.org/2001/XMLSchema#> .
@prefix owl: <http://www.w3.org/2002/07/owl#>
@prefix skos: <http://www.w3.org/2004/02/skos/core#> 
@prefix :   <https://w3id.org/EnergyInformationModel/profiles/ontologyprofile/ontologyshape#> .





################################################################
####  sh:NodeShapes
###############################################################
:ClassShape
    a sh:NodeShape ;
    sh:targetClass owl:Class ;
    sh:property :PrefLabelShape ;
    sh:property :DefinitionShape.
    
:ObjectPropertyShape
    a sh:NodeShape ;
    sh:targetClass owl:ObjectProperty ;
    sh:property :PrefLabelShape ;
    sh:property :DefinitionShape ;
    sh:property :DomainShape
    sh:property [
        rdfs:comment "At least one range is defined to ensure correct transformation to OO artifacts"@en;
        sh:path rdfs:range ;
        sh:node :ClassShape ;
        sh:minCount 1 ;
    ] .



:DatatypePropertyShape
    a sh:NodeShape ;
    sh:targetClass owl:DatatypeProperty ;
    sh:property :PrefLabelShape ;
    sh:property :DefinitionShape ;
    sh:property [
        rdfs:comment "At least one range is defined to ensure correct transformation to OO artifacts"@en;
        sh:path rdfs:range ;
        sh:minCount 1 ;
    ].


################################################################
####  sh:PropertyShapes
###############################################################


:PrefLabelShape 
    a sh:PropertyShape   ;
    rdfs:comment "Any class has at most one prefLabel for each language, each class has at least one prefLabel in one language"@en;
    sh:path skos:prefLabel ;
    sh:datatype xsd:string ;
    sh:minCount 1 .

:DefinitionShape 
    a sh:PropertyShape ;
    rdfs:comment "Any resource has at least one definition in one language"@en ;
    sh:path skos:definition ;
    sh:datatype xsd:string ;
    sh:minCount 1 .

:DomainShape 
    a sh:PropertyShape ;
    rdfs:comment "At least one domain is defined to ensure correct transformation to OO artifacts"@en;
    sh:path rdfs:domain ;
    sh:node :ClassShape ;
    sh:minCount 1 ;
>>>>>>> f95fee49c3f80112da44df26d0295ef06e89e5e7
