@prefix : <https://w3id.org/EnergyInformationModel/ontology/network/primarycomponents#> .
@prefix owl: <http://www.w3.org/2002/07/owl#> .
@prefix rdf: <http://www.w3.org/1999/02/22-rdf-syntax-ns#> .
@prefix xml: <http://www.w3.org/XML/1998/namespace> .
@prefix xsd: <http://www.w3.org/2001/XMLSchema#> .
@prefix eimc: <https://w3id.org/energyinformationmodel/ontology/core#> .
@prefix rdfs: <http://www.w3.org/2000/01/rdf-schema#> .
@prefix eimpc: <https://w3id.org/EnergyInformationModel/ontology/network/primarycomponents#> .
@base <https://w3id.org/EnergyInformationModel/ontology/network/primarycomponents#> .

<https://w3id.org/EnergyInformationModel/ontology/network/primarycomponents#> rdf:type owl:Ontology ;
                                                                               owl:imports <https://w3id.org/EnergyInformationModel/ontology/core#> ;
                                                                               <http://purl.org/dc/terms/conformsTo> <https://w3id.org/EnergyInformationModel/profiles/ontologyprofile/ontologyshape#> ;
                                                                               <http://purl.org/dc/terms/license> <https://www.apache.org/licenses/LICENSE-2.0> ;
                                                                               <http://purl.org/dc/terms/requires> <https://w3id.org/EnergyInformationModel/ontology/core#> ;
                                                                               rdfs:comment "The Primary Component ontology in the Energy Information model defines the components of an energy system that carry the energy for the purpose of transport and distribution."@en ;
                                                                               rdfs:seeAlso <http://www.iec.ch/TC57/CIM#> .

#################################################################
#    Annotation properties
#################################################################

###  http://purl.org/dc/terms/conformsTo
<http://purl.org/dc/terms/conformsTo> rdf:type owl:AnnotationProperty .


###  http://purl.org/dc/terms/license
<http://purl.org/dc/terms/license> rdf:type owl:AnnotationProperty .


###  http://purl.org/dc/terms/requires
<http://purl.org/dc/terms/requires> rdf:type owl:AnnotationProperty .


###  http://www.w3.org/2004/02/skos/core#definition
<http://www.w3.org/2004/02/skos/core#definition> rdf:type owl:AnnotationProperty .


###  http://www.w3.org/2004/02/skos/core#editorialNote
<http://www.w3.org/2004/02/skos/core#editorialNote> rdf:type owl:AnnotationProperty .


###  http://www.w3.org/2004/02/skos/core#prefLabel
<http://www.w3.org/2004/02/skos/core#prefLabel> rdf:type owl:AnnotationProperty .


#################################################################
#    Object Properties
#################################################################

###  https://w3id.org/EnergyInformationModel/ontology/core#383fc6ce_402d_4c81_a4e8_dea9613d7a3e
<https://w3id.org/EnergyInformationModel/ontology/core#383fc6ce_402d_4c81_a4e8_dea9613d7a3e> rdf:type owl:ObjectProperty .


###  https://w3id.org/EnergyInformationModel/ontology/core#95194981_485f_4850_b1b3_d6e684529a99
<https://w3id.org/EnergyInformationModel/ontology/core#95194981_485f_4850_b1b3_d6e684529a99> rdf:type owl:ObjectProperty .


###  https://w3id.org/EnergyInformationModel/ontology/network/primarycomponents#f4817738_268e_47ab_bd9f_070880fa1d9f
eimpc:f4817738_268e_47ab_bd9f_070880fa1d9f rdf:type owl:ObjectProperty ;
                                           rdfs:subPropertyOf <https://w3id.org/EnergyInformationModel/ontology/core#95194981_485f_4850_b1b3_d6e684529a99> ;
                                           owl:inverseOf <https://w3id.org/EnergyInformationModel/ontology/network/primarycomponents#78ce8fb9_61e5_4bd3_8453_c93d9da4a6f4> ;
                                           rdfs:domain <https://w3id.org/EnergyInformationModel/ontology/network/primarycomponents#6b198bd1_3cd5_449b_9447_23f7fa839b52> ;
                                           rdfs:range <https://w3id.org/EnergyInformationModel/ontology/network/primarycomponents#521235f9_146a_40f6_951a_04f0b06b2aa2> ;
                                           <http://www.w3.org/2004/02/skos/core#definition> "Relates the Transformer to its TransformerEnds"@en ;
                                           <http://www.w3.org/2004/02/skos/core#prefLabel> "HasTransformerEnds"@en .


###  https://w3id.org/EnergyInformationModel/ontology/network/primarycomponents#fbaaff7e_67eb_45b7_882a_1f3d166ab849
eimpc:fbaaff7e_67eb_45b7_882a_1f3d166ab849 rdf:type owl:ObjectProperty ;
                                           rdfs:domain <https://w3id.org/EnergyInformationModel/ontology/network/primarycomponents#1f327447_2de1_412e_bb40_1e548aed4467> ;
                                           rdfs:range <https://w3id.org/EnergyInformationModel/ontology/core#defcdc40_e2ec_4174_b9c8_a60992fdb317> ;
                                           <http://www.w3.org/2004/02/skos/core#definition> "Relates Primary Equipment and TopologicalNodes to the operational envelope at which they are operated"@en ;
                                           <http://www.w3.org/2004/02/skos/core#prefLabel> "OperatedAt"@en .


###  https://w3id.org/EnergyInformationModel/ontology/network/primarycomponents#4d45d15d_4e95_4ecf_842e_70c49e78afca
<https://w3id.org/EnergyInformationModel/ontology/network/primarycomponents#4d45d15d_4e95_4ecf_842e_70c49e78afca> rdf:type owl:ObjectProperty ;
                                                                                                                  rdfs:domain <https://w3id.org/EnergyInformationModel/ontology/network/primarycomponents#521235f9_146a_40f6_951a_04f0b06b2aa2> ;
                                                                                                                  rdfs:range eimc:a8bec9fa_deb6_4fe9_8726_0b8b6208fa73 ;
                                                                                                                  <http://www.w3.org/2004/02/skos/core#definition> "Relates the TransformerEnd to one of the terminals of a Transformer so that it can be placed acurately  in a Network Model."@en ;
                                                                                                                  <http://www.w3.org/2004/02/skos/core#prefLabel> "AtTerminal"@en .


###  https://w3id.org/EnergyInformationModel/ontology/network/primarycomponents#429f58a7_9065_4c0e_a2a3_009761f78b7e
<https://w3id.org/EnergyInformationModel/ontology/network/primarycomponents#429f58a7_9065_4c0e_a2a3_009761f78b7e> rdf:type owl:ObjectProperty ;
                                                                                                                  rdfs:domain <https://w3id.org/EnergyInformationModel/ontology/network/primarycomponents#1f327447_2de1_412e_bb40_1e548aed4467> ;
                                                                                                                  rdfs:range eimc:a8bec9fa_deb6_4fe9_8726_0b8b6208fa73 ;
                                                                                                                  <http://www.w3.org/2004/02/skos/core#definition> "Relates a Primary Equipment to its Terminals."@en ;
                                                                                                                  <http://www.w3.org/2004/02/skos/core#prefLabel> "HasTerminals"@en .


###  https://w3id.org/EnergyInformationModel/ontology/network/primarycomponents#78ce8fb9_61e5_4bd3_8453_c93d9da4a6f4
<https://w3id.org/EnergyInformationModel/ontology/network/primarycomponents#78ce8fb9_61e5_4bd3_8453_c93d9da4a6f4> rdf:type owl:ObjectProperty ;
                                                                                                                  rdfs:subPropertyOf <https://w3id.org/EnergyInformationModel/ontology/core#383fc6ce_402d_4c81_a4e8_dea9613d7a3e> ;
                                                                                                                  rdfs:domain <https://w3id.org/EnergyInformationModel/ontology/network/primarycomponents#521235f9_146a_40f6_951a_04f0b06b2aa2> ;
                                                                                                                  rdfs:range <https://w3id.org/EnergyInformationModel/ontology/network/primarycomponents#6b198bd1_3cd5_449b_9447_23f7fa839b52> ;
                                                                                                                  <http://www.w3.org/2004/02/skos/core#definition> "Relates the Transformer to which the TransformerEnd belongs."@en ;
                                                                                                                  <http://www.w3.org/2004/02/skos/core#prefLabel> "PartOfTransformer"@en .


#################################################################
#    Data properties
#################################################################

###  https://w3id.org/EnergyInformationModel/ontology/network/primarycomponents#53e95c7e_a2ff_480a_9557_fa4df0d1b1be
<https://w3id.org/EnergyInformationModel/ontology/network/primarycomponents#53e95c7e_a2ff_480a_9557_fa4df0d1b1be> rdf:type owl:DatatypeProperty ;
                                                                                                                  rdfs:domain <https://w3id.org/EnergyInformationModel/ontology/network/primarycomponents#75a82637_c3d3_44b6_af30_37f3a56a4dfb> ;
                                                                                                                  rdfs:range xsd:boolean ;
                                                                                                                  <http://www.w3.org/2004/02/skos/core#definition> """. Indicates whether the Disconnector currently allows energy to flow through. Value of True means energy can pass through, value of False means energy flow is interrupted.

N.B. This definition is a Simplified version of the disconnector status that may be used for evaluating scenario's.
For master data and archival purposes, the DisconnectorStatus should be used"""@en ;
                                                                                                                  <http://www.w3.org/2004/02/skos/core#prefLabel> "currentlyConnecting"@en .


#################################################################
#    Classes
#################################################################

###  http://www.iec.ch/TC57/CIM#IdentifiedObject
<http://www.iec.ch/TC57/CIM#IdentifiedObject> rdf:type owl:Class .


###  https://w3id.org/EnergyInformationModel/ontology/core#2cd0f6fc_b577_427f_95bd_8dd439350c82
<https://w3id.org/EnergyInformationModel/ontology/core#2cd0f6fc_b577_427f_95bd_8dd439350c82> rdf:type owl:Class .


###  https://w3id.org/EnergyInformationModel/ontology/network/primarycomponents#f4574df8_5829_485f_8481_0f5a15a85eac
eimpc:f4574df8_5829_485f_8481_0f5a15a85eac rdf:type owl:Class ;
                                           rdfs:subClassOf <https://w3id.org/EnergyInformationModel/ontology/network/primarycomponents#1f327447_2de1_412e_bb40_1e548aed4467> ;
                                           <http://www.w3.org/2004/02/skos/core#definition> "A primary equipment or group of primary equipment with negligible energy loss that serve to connect other primary equipmen and are modelled with a single logical terminal."@en ;
                                           <http://www.w3.org/2004/02/skos/core#editorialNote> "Generic energy system definition for http://www.iec.ch/TC57/CIM#Connector"@en ;
                                           <http://www.w3.org/2004/02/skos/core#prefLabel> "Connector"@en ,
                                                                                           "Koppelfunctie"@nl .


###  https://w3id.org/EnergyInformationModel/ontology/network/primarycomponents#1f327447_2de1_412e_bb40_1e548aed4467
<https://w3id.org/EnergyInformationModel/ontology/network/primarycomponents#1f327447_2de1_412e_bb40_1e548aed4467> rdf:type owl:Class ;
                                                                                                                  rdfs:subClassOf <https://w3id.org/EnergyInformationModel/ontology/core#2cd0f6fc_b577_427f_95bd_8dd439350c82> ;
                                                                                                                  <http://www.w3.org/2004/02/skos/core#definition> "Equipment that form the primary components of an energy infrastructure."@nl ;
                                                                                                                  <http://www.w3.org/2004/02/skos/core#editorialNote> "Generic energy system definition of http://www.iec.ch/TC57/CIM#ConductingEquipment"@en ;
                                                                                                                  <http://www.w3.org/2004/02/skos/core#prefLabel> "PrimaryEquipment"@en .


###  https://w3id.org/EnergyInformationModel/ontology/network/primarycomponents#385be6d9_0eef_4d6c_82f9_af39e756dca9
<https://w3id.org/EnergyInformationModel/ontology/network/primarycomponents#385be6d9_0eef_4d6c_82f9_af39e756dca9> rdf:type owl:Class ;
                                                                                                                  rdfs:subClassOf <https://w3id.org/EnergyInformationModel/ontology/network/primarycomponents#6b198bd1_3cd5_449b_9447_23f7fa839b52> ;
                                                                                                                  <http://www.w3.org/2004/02/skos/core#definition> "An FuelCell a device that transforms Hydrogen (or sometimes other fuels) into Electricity . For the purpose of energy system analyses, it is a type of transformer, with one TransformerEnd in the Hydrogen domain, where it behaves a s a sink, and one TransformerEnd in the electricity domain where it behaves as a source."@en ;
                                                                                                                  <http://www.w3.org/2004/02/skos/core#prefLabel> "FuelCell"@en .


###  https://w3id.org/EnergyInformationModel/ontology/network/primarycomponents#416cebbf_6714_4051_a7b8_171d015d2b92
<https://w3id.org/EnergyInformationModel/ontology/network/primarycomponents#416cebbf_6714_4051_a7b8_171d015d2b92> rdf:type owl:Class ;
                                                                                                                  rdfs:subClassOf <https://w3id.org/EnergyInformationModel/ontology/network/primarycomponents#6b198bd1_3cd5_449b_9447_23f7fa839b52> ;
                                                                                                                  <http://www.w3.org/2004/02/skos/core#definition> "An Electrolyser is a device that transforms electricity into hydrogen. For the purpose of energy system analyses, it is a type of transformer, with one TransformerEnd in the electricity domain, where it behaves a s a sink, and one TransformerEnd in the hydrogen domain where it behaves as a source."@en ;
                                                                                                                  <http://www.w3.org/2004/02/skos/core#prefLabel> "Electrolyser"@en .


###  https://w3id.org/EnergyInformationModel/ontology/network/primarycomponents#521235f9_146a_40f6_951a_04f0b06b2aa2
<https://w3id.org/EnergyInformationModel/ontology/network/primarycomponents#521235f9_146a_40f6_951a_04f0b06b2aa2> rdf:type owl:Class ;
                                                                                                                  rdfs:subClassOf <http://www.iec.ch/TC57/CIM#IdentifiedObject> ;
                                                                                                                  <http://www.w3.org/2004/02/skos/core#definition> """Transformers tansform the nature of the energy that passes through them. The TransformerEnd defines the 'side' of the transformer and therefore can be associated with a certain state variable.

Examples include the 
- high-voltage and low-voltage sides of a Power Transformer 
- High pressure and the low pressure sides of of a compressor
- the electric and hydrogen side of a fuel cell"""@en ;
                                                                                                                  <http://www.w3.org/2004/02/skos/core#prefLabel> "TransformerEnd"@en .


###  https://w3id.org/EnergyInformationModel/ontology/network/primarycomponents#6b198bd1_3cd5_449b_9447_23f7fa839b52
<https://w3id.org/EnergyInformationModel/ontology/network/primarycomponents#6b198bd1_3cd5_449b_9447_23f7fa839b52> rdf:type owl:Class ;
                                                                                                                  rdfs:subClassOf <https://w3id.org/EnergyInformationModel/ontology/network/primarycomponents#1f327447_2de1_412e_bb40_1e548aed4467> ;
                                                                                                                  <http://www.w3.org/2004/02/skos/core#definition> "Primary equipment that intentionally alters the state variables or form of energy. Examples include Power Transformers. Compressors or Fuel Cells."@en ;
                                                                                                                  <http://www.w3.org/2004/02/skos/core#editorialNote> "Generic energy system definition of http://www.iec.ch/TC57/CIM#PowerTransformer"@en ;
                                                                                                                  <http://www.w3.org/2004/02/skos/core#prefLabel> "Transformatiefunctie"@nl ,
                                                                                                                                                                  "Transformer"@en .


###  https://w3id.org/EnergyInformationModel/ontology/network/primarycomponents#7c5f4ddf_4467_4c72_b26b_4c96485bd533
<https://w3id.org/EnergyInformationModel/ontology/network/primarycomponents#7c5f4ddf_4467_4c72_b26b_4c96485bd533> rdf:type owl:Class ;
                                                                                                                  rdfs:subClassOf <https://w3id.org/EnergyInformationModel/ontology/network/primarycomponents#1f327447_2de1_412e_bb40_1e548aed4467> ;
                                                                                                                  <http://www.w3.org/2004/02/skos/core#definition> """Primary equipment, with uniform properties with regard to energy loss, used for transporting energy over a distance. 

Examples include cable segments in electricity- or pipesegments in gas infrastructure"""@en ;
                                                                                                                  <http://www.w3.org/2004/02/skos/core#editorialNote> "Generic energy system definition of http://www.iec.ch/TC57/CIM#Conductor"@en ;
                                                                                                                  <http://www.w3.org/2004/02/skos/core#prefLabel> "Transporter"@en ,
                                                                                                                                                                  "Transportfunctie"@nl .


###  https://w3id.org/EnergyInformationModel/ontology/network/primarycomponents#75a82637_c3d3_44b6_af30_37f3a56a4dfb
<https://w3id.org/EnergyInformationModel/ontology/network/primarycomponents#75a82637_c3d3_44b6_af30_37f3a56a4dfb> rdf:type owl:Class ;
                                                                                                                  rdfs:subClassOf <https://w3id.org/EnergyInformationModel/ontology/network/primarycomponents#1f327447_2de1_412e_bb40_1e548aed4467> ;
                                                                                                                  <http://www.w3.org/2004/02/skos/core#definition> "Generic device for interrupting energy flow through a system. Examples include Swtiches annd Valves"@en ;
                                                                                                                  <http://www.w3.org/2004/02/skos/core#editorialNote> "Generic energy system definition of http://www.iec.ch/TC57/CIM#Switch"@en ;
                                                                                                                  <http://www.w3.org/2004/02/skos/core#prefLabel> "Disconnector"@en ,
                                                                                                                                                                  "Onderbrekerfunctie"@nl .


###  https://w3id.org/EnergyInformationModel/ontology/network/primarycomponents#84c50d0d_8ee4_41b2_b793_667e7e62c53f
<https://w3id.org/EnergyInformationModel/ontology/network/primarycomponents#84c50d0d_8ee4_41b2_b793_667e7e62c53f> rdf:type owl:Class ;
                                                                                                                  rdfs:subClassOf <https://w3id.org/EnergyInformationModel/ontology/network/primarycomponents#1f327447_2de1_412e_bb40_1e548aed4467> ;
                                                                                                                  <http://www.w3.org/2004/02/skos/core#definition> "A point in the system where energy can be let out for the purpose of safely working on the system. Examples include Ground and Vent."@en ;
                                                                                                                  <http://www.w3.org/2004/02/skos/core#editorialNote> "Generic energy system definition of http://www.iec.ch/TC57/CIM#Ground"@en ;
                                                                                                                  <http://www.w3.org/2004/02/skos/core#prefLabel> "DeEnergizer"@en ,
                                                                                                                                                                  "Energielozingfunctie"@nl .


###  https://w3id.org/energyinformationmodel/ontology/core#a8bec9fa_deb6_4fe9_8726_0b8b6208fa73
eimc:a8bec9fa_deb6_4fe9_8726_0b8b6208fa73 rdf:type owl:Class .


###  Generated by the OWL API (version 4.5.9.2019-02-01T07:24:44Z) https://github.com/owlcs/owlapi
