@prefix : <https://w3id.org/EnergyInformationModel/ontology/core#> .
@prefix owl: <http://www.w3.org/2002/07/owl#> .
@prefix rdf: <http://www.w3.org/1999/02/22-rdf-syntax-ns#> .
@prefix xml: <http://www.w3.org/XML/1998/namespace> .
@prefix xsd: <http://www.w3.org/2001/XMLSchema#> .
@prefix eimc: <https://w3id.org/energyinformationmodel/ontology/core> .
@prefix rdfs: <http://www.w3.org/2000/01/rdf-schema#> .

<https://w3id.org/EnergyInformationModel/ontology/core#> a owl:Ontology ;
	<http://purl.org/dc/terms/conformsTo> <https://w3id.org/EnergyInformationModel/profiles/ontologyprofile/ontologyshape#> ;
	rdfs:comment "Core concept ontology for the Energy Information Model" ;
	rdfs:seeAlso <http://www.iec.ch/TC57/CIM#> .
# 
# 
# #################################################################
# #
# #    Annotation properties
# #
# #################################################################
# 
# 
# http://purl.org/dc/terms/conformsTo

<http://purl.org/dc/terms/conformsTo> a owl:AnnotationProperty .
# 
# http://www.w3.org/2004/02/skos/core#definition

<http://www.w3.org/2004/02/skos/core#definition> a owl:AnnotationProperty .
# 
# http://www.w3.org/2004/02/skos/core#editorialNote

<http://www.w3.org/2004/02/skos/core#editorialNote> a owl:AnnotationProperty .
# 
# http://www.w3.org/2004/02/skos/core#prefLabel

<http://www.w3.org/2004/02/skos/core#prefLabel> a owl:AnnotationProperty .
# 
# 
# 
# #################################################################
# #
# #    Object Properties
# #
# #################################################################
# 
# 
# https://w3id.org/EnergyInformationModel/ontology/core#ab69031a_06aa_4087_9795_3f99cfe5dc87

:ab69031a_06aa_4087_9795_3f99cfe5dc87 a owl:ObjectProperty ;
	rdfs:subPropertyOf :95194981_485f_4850_b1b3_d6e684529a99 ;
	owl:inverseOf :1dcddd6a_e404_455a_b672_a61c6d44f16e ;
	rdfs:domain :775ccc29_5e85_4aa3_87ad_21cfac22dbec ;
	rdfs:range <https://w3id.org/energyinformationmodel/ontology/core#b54a2641_b1fa_46d4_8bd5_24161660e542> ;
	<http://www.w3.org/2004/02/skos/core#definition> "Relates the container to the ConnectivityNodes it contains."@en ;
	<http://www.w3.org/2004/02/skos/core#prefLabel> "ContainsConnectivityNodes"@en .
# 
# https://w3id.org/EnergyInformationModel/ontology/core#aba85ef3_f3a2_4164_98d3_dfe8b030908c

:aba85ef3_f3a2_4164_98d3_dfe8b030908c a owl:ObjectProperty ;
	rdfs:subPropertyOf :95194981_485f_4850_b1b3_d6e684529a99 ;
	owl:inverseOf :41485cfe_3c29_4250_aea1_29a0c50eb639 ;
	rdfs:domain :38ad6b49_857f_41f0_b591_77722ee25269 ;
	rdfs:range :2cd0f6fc_b577_427f_95bd_8dd439350c82 ;
	<http://www.w3.org/2004/02/skos/core#definition> "Relates the container to the equipment it contains"@en ;
	<http://www.w3.org/2004/02/skos/core#prefLabel> "ContainsEquipment"@en .
# 
# https://w3id.org/EnergyInformationModel/ontology/core#1dcddd6a_e404_455a_b672_a61c6d44f16e

:1dcddd6a_e404_455a_b672_a61c6d44f16e a owl:ObjectProperty ;
	rdfs:subPropertyOf :383fc6ce_402d_4c81_a4e8_dea9613d7a3e ;
	rdfs:domain <https://w3id.org/energyinformationmodel/ontology/core#b54a2641_b1fa_46d4_8bd5_24161660e542> ;
	rdfs:range :775ccc29_5e85_4aa3_87ad_21cfac22dbec ;
	<http://www.w3.org/2004/02/skos/core#definition> "Relates the ConnectivityNode to the containers it is part of"@en ;
	<http://www.w3.org/2004/02/skos/core#prefLabel> "PartOfConnectivityNodeContainer"@en .
# 
# https://w3id.org/EnergyInformationModel/ontology/core#383fc6ce_402d_4c81_a4e8_dea9613d7a3e

:383fc6ce_402d_4c81_a4e8_dea9613d7a3e a owl:ObjectProperty ;
	owl:inverseOf :95194981_485f_4850_b1b3_d6e684529a99 ;
	a owl:TransitiveProperty ;
	rdfs:domain owl:Thing ;
	rdfs:range owl:Thing ;
	rdfs:seeAlso <https://www.w3.org/2001/sw/BestPractices/OEP/SimplePartWhole/> ;
	<http://www.w3.org/2004/02/skos/core#definition> "Relate the parts to a larger thing that they are part of."@en ;
	<http://www.w3.org/2004/02/skos/core#prefLabel> "PartOf"@en .
# 
# https://w3id.org/EnergyInformationModel/ontology/core#41485cfe_3c29_4250_aea1_29a0c50eb639

:41485cfe_3c29_4250_aea1_29a0c50eb639 a owl:ObjectProperty ;
	rdfs:subPropertyOf :383fc6ce_402d_4c81_a4e8_dea9613d7a3e ;
	rdfs:domain :2cd0f6fc_b577_427f_95bd_8dd439350c82 ;
	rdfs:range :775ccc29_5e85_4aa3_87ad_21cfac22dbec ;
	<http://www.w3.org/2004/02/skos/core#definition> "Relates equipment to the equipment container it is part of"@en ;
	<http://www.w3.org/2004/02/skos/core#prefLabel> "PartOfEquipmentContainer"@en .
# 
# https://w3id.org/EnergyInformationModel/ontology/core#89c544c0_b500_43e6_aa90_21cb601172a7

:89c544c0_b500_43e6_aa90_21cb601172a7 a owl:ObjectProperty ;
	owl:inverseOf <https://w3id.org/EnergyInformationModel/ontology/network/primarycomponents#429f58a7_9065_4c0e_a2a3_009761f78b7e> ;
	rdfs:domain <https://w3id.org/energyinformationmodel/ontology/core#a8bec9fa_deb6_4fe9_8726_0b8b6208fa73> ;
	rdfs:range <https://w3id.org/EnergyInformationModel/ontology/network/primarycomponents#1f327447_2de1_412e_bb40_1e548aed4467> ;
	<http://www.w3.org/2004/02/skos/core#definition> "Relates the terminal to the Primary Equipment it belongs to."@en ;
	<http://www.w3.org/2004/02/skos/core#prefLabel> "BelongsToPrimaryEquipment"@en .
# 
# https://w3id.org/EnergyInformationModel/ontology/core#95194981_485f_4850_b1b3_d6e684529a99

:95194981_485f_4850_b1b3_d6e684529a99 a owl:ObjectProperty ;
	rdfs:subPropertyOf owl:topObjectProperty ;
	a owl:TransitiveProperty ;
	rdfs:domain owl:Thing ;
	rdfs:range owl:Thing ;
	rdfs:seeAlso <https://www.w3.org/2001/sw/BestPractices/OEP/SimplePartWhole/> ;
	<http://www.w3.org/2004/02/skos/core#definition> "Relates a thing to its parts in the context of a decomposition."@en ;
	<http://www.w3.org/2004/02/skos/core#prefLabel> "HasPart"@en .
# 
# https://w3id.org/EnergyInformationModel/ontology/network/primarycomponents#429f58a7_9065_4c0e_a2a3_009761f78b7e

<https://w3id.org/EnergyInformationModel/ontology/network/primarycomponents#429f58a7_9065_4c0e_a2a3_009761f78b7e> a owl:ObjectProperty ;
	<http://www.w3.org/2004/02/skos/core#prefLabel> "HasTerminal"@en .
# 
# https://w3id.org/energyinformationmodel/ontology/core#c88cde8a_ebcc_483f_9e64_e76f095d7e0e

<https://w3id.org/energyinformationmodel/ontology/core#c88cde8a_ebcc_483f_9e64_e76f095d7e0e> a owl:ObjectProperty ;
	owl:inverseOf <https://w3id.org/energyinformationmodel/ontology/core#989c262b_4f54_4b2d_b9eb_5c92bf81ec7a> ;
	rdfs:domain <https://w3id.org/energyinformationmodel/ontology/core#c277f37c_c697_4522_9558_16d98edb8ab1> ;
	rdfs:range <http://www.iec.ch/TC57/CIM#Asset> ;
	<http://www.w3.org/2004/02/skos/core#definition> "Relates the energy system resource to the asset that implements it."@en ;
	<http://www.w3.org/2004/02/skos/core#prefLabel> "ImplementedByAsset"@en .
# 
# https://w3id.org/energyinformationmodel/ontology/core#dc955e18_f1c8_4c8b_8f4a_d41565526307

<https://w3id.org/energyinformationmodel/ontology/core#dc955e18_f1c8_4c8b_8f4a_d41565526307> a owl:ObjectProperty ;
	owl:inverseOf <https://w3id.org/energyinformationmodel/ontology/core#43bdc0e6_3c6d_4d85_b7c1_4a5bc0e93812> ;
	rdfs:domain <https://w3id.org/energyinformationmodel/ontology/core#a8bec9fa_deb6_4fe9_8726_0b8b6208fa73> ;
	rdfs:range <https://w3id.org/energyinformationmodel/ontology/core#b54a2641_b1fa_46d4_8bd5_24161660e542> ;
	<http://www.w3.org/2004/02/skos/core#definition> "Defines the relationship to the connectivity node that this terminal is connected to"@en ;
	<http://www.w3.org/2004/02/skos/core#prefLabel> "ConnectsConnectivityNode"@en .
# 
# https://w3id.org/energyinformationmodel/ontology/core#43bdc0e6_3c6d_4d85_b7c1_4a5bc0e93812

<https://w3id.org/energyinformationmodel/ontology/core#43bdc0e6_3c6d_4d85_b7c1_4a5bc0e93812> a owl:ObjectProperty ;
	rdfs:domain <https://w3id.org/energyinformationmodel/ontology/core#b54a2641_b1fa_46d4_8bd5_24161660e542> ;
	rdfs:range <https://w3id.org/energyinformationmodel/ontology/core#a8bec9fa_deb6_4fe9_8726_0b8b6208fa73> ;
	<http://www.w3.org/2004/02/skos/core#definition> "The relationship that defines the terminals that are connected through this connectivity node"@en ;
	<http://www.w3.org/2004/02/skos/core#prefLabel> "ConnectsTerminals"@en .
# 
# https://w3id.org/energyinformationmodel/ontology/core#989c262b_4f54_4b2d_b9eb_5c92bf81ec7a

<https://w3id.org/energyinformationmodel/ontology/core#989c262b_4f54_4b2d_b9eb_5c92bf81ec7a> a owl:ObjectProperty ;
	rdfs:domain <http://www.iec.ch/TC57/CIM#Asset> ;
	rdfs:range <https://w3id.org/energyinformationmodel/ontology/core#c277f37c_c697_4522_9558_16d98edb8ab1> ;
	<http://www.w3.org/2004/02/skos/core#prefLabel> "ImplementsFunction"@en .
# 
# 
# 
# #################################################################
# #
# #    Data properties
# #
# #################################################################
# 
# 
# http://www.iec.ch/TC57/CIM#IdentifiedObject.mRID

<http://www.iec.ch/TC57/CIM#IdentifiedObject.mRID> a owl:DatatypeProperty ;
	rdfs:domain <http://www.iec.ch/TC57/CIM#IdentifiedObject> ;
	rdfs:range xsd:string ;
	rdfs:isDefinedBy <http://www.iec.ch/TC57/CIM#> ;
	<http://www.w3.org/2004/02/skos/core#definition> "Master resource identifier issued by a data authority. The mRID is unique within an exchange context. Global uniqueness is easily achieved by using a UUID as specified in RFC 4122 for the mRID. The use of UUID is strongly recommended." ;
	<http://www.w3.org/2004/02/skos/core#prefLabel> "mRID" .
# 
# 
# 
# #################################################################
# #
# #    Classes
# #
# #################################################################
# 
# 
# http://www.iec.ch/TC57/CIM#Asset

<http://www.iec.ch/TC57/CIM#Asset> a owl:Class ;
	rdfs:subClassOf <http://www.iec.ch/TC57/CIM#IdentifiedObject> ;
	owl:disjointWith <https://w3id.org/energyinformationmodel/ontology/core#c277f37c_c697_4522_9558_16d98edb8ab1> ;
	rdfs:isDefinedBy <http://www.iec.ch/TC57/CIM#> ;
	<http://www.w3.org/2004/02/skos/core#definition> """Tangible resource of the utility including energy system equipment various end devices cabinets buildings etc. For energy network equipment the role of the asset is defined through EnergySystemResource and its subclasses. Asset description places emphasis on the physical characteristics of the equipment fulfilling that role.

An Asset typically comes into exsistence during a production process (whether at a production site or in the field) and seizes to exist when it is permanently disassembled, landfilled or recycled. When an asset is reused, it retains it identity."""@en ;
	<http://www.w3.org/2004/02/skos/core#prefLabel> "Asset"@en .
# 
# http://www.iec.ch/TC57/CIM#IdentifiedObject

<http://www.iec.ch/TC57/CIM#IdentifiedObject> a owl:Class ;
	rdfs:isDefinedBy <http://www.iec.ch/TC57/CIM#> ;
	rdfs:label "Geïdentificeerd Object"@nl ;
	<http://www.w3.org/2004/02/skos/core#definition> "This is a root class to provide common identification for all classes needing identification and naming attributes."@en ;
	<http://www.w3.org/2004/02/skos/core#prefLabel> "IdentifiedObject"@en .
# 
# https://w3id.org/EnergyInformationModel/ontology/core#c1105b1a_0b23_4e62_8ef0_7db16771cc72

:c1105b1a_0b23_4e62_8ef0_7db16771cc72 a owl:Class ;
	<http://www.w3.org/2004/02/skos/core#definition> "Defines the domain to which the energy system belongs. Examples include, Electricity, Natural Gas and Hydrogen" ;
	<http://www.w3.org/2004/02/skos/core#prefLabel> "EnergyDomain"@en .
# 
# https://w3id.org/EnergyInformationModel/ontology/core#defcdc40_e2ec_4174_b9c8_a60992fdb317

:defcdc40_e2ec_4174_b9c8_a60992fdb317 a owl:Class ;
	rdfs:subClassOf <http://www.iec.ch/TC57/CIM#IdentifiedObject> ;
	<http://www.w3.org/2004/02/skos/core#definition> "Defines the Operational Envelope at which a part of the grid is operated. In electricity (AC) this is typically expressed with a Voltage Level and a frequency, In Gas this typoically involves Caloric Value and Pressure level."@en ;
	<http://www.w3.org/2004/02/skos/core#prefLabel> "OperationalEnvelope"@en .
# 
# https://w3id.org/EnergyInformationModel/ontology/core#2cd0f6fc_b577_427f_95bd_8dd439350c82

:2cd0f6fc_b577_427f_95bd_8dd439350c82 a owl:Class ;
	rdfs:subClassOf <https://w3id.org/energyinformationmodel/ontology/core#c277f37c_c697_4522_9558_16d98edb8ab1> ;
	<http://www.w3.org/2004/02/skos/core#definition> "Smallest functional elements in an energy system. Examples include Switches, Valves, BusbarSections, or T-sections."@en ;
	<http://www.w3.org/2004/02/skos/core#prefLabel> "Equipment"@en .
# 
# https://w3id.org/EnergyInformationModel/ontology/core#38ad6b49_857f_41f0_b591_77722ee25269

:38ad6b49_857f_41f0_b591_77722ee25269 a owl:Class ;
	rdfs:subClassOf :775ccc29_5e85_4aa3_87ad_21cfac22dbec ;
	<http://www.w3.org/2004/02/skos/core#definition> "A modelling construct to provide a root class for containing equipment."@en ;
	<http://www.w3.org/2004/02/skos/core#editorialNote> "Generic energy system definition of http://www.iec.ch/TC57/CIM#EquipmentContainer"@en ;
	<http://www.w3.org/2004/02/skos/core#prefLabel> "EquipmentContainer"@en .
# 
# https://w3id.org/EnergyInformationModel/ontology/core#775ccc29_5e85_4aa3_87ad_21cfac22dbec

:775ccc29_5e85_4aa3_87ad_21cfac22dbec a owl:Class ;
	rdfs:subClassOf <https://w3id.org/energyinformationmodel/ontology/core#c277f37c_c697_4522_9558_16d98edb8ab1> ;
	<http://www.w3.org/2004/02/skos/core#definition> "A base class for all objects that may contain connectivity nodes or topological nodes."@en ;
	<http://www.w3.org/2004/02/skos/core#editorialNote> "generic energysystem definition of http://www.iec.ch/TC57/CIM#ConnectivityNodeContainer"@en ;
	<http://www.w3.org/2004/02/skos/core#prefLabel> "ConnectivityNodeContainer"@en .
# 
# https://w3id.org/EnergyInformationModel/ontology/core#90b72f14_5778_4138_a42c_2115426699d3

:90b72f14_5778_4138_a42c_2115426699d3 a owl:Class ;
	rdfs:subClassOf :38ad6b49_857f_41f0_b591_77722ee25269 ;
	<http://www.w3.org/2004/02/skos/core#definition> "A collection of equipment for purposes other than generation or utilization through which energy in bulk is passed for the purposes of switching or modifying its characteristics."@en ;
	<http://www.w3.org/2004/02/skos/core#editorialNote> "Generic energy system definition for http://www.iec.ch/TC57/CIM#Substation"@en ;
	<http://www.w3.org/2004/02/skos/core#prefLabel> "Substation"@en .
# 
# https://w3id.org/EnergyInformationModel/ontology/network/primarycomponents#1f327447_2de1_412e_bb40_1e548aed4467

<https://w3id.org/EnergyInformationModel/ontology/network/primarycomponents#1f327447_2de1_412e_bb40_1e548aed4467> a owl:Class ;
	rdfs:subClassOf :2cd0f6fc_b577_427f_95bd_8dd439350c82 ;
	<http://www.w3.org/2004/02/skos/core#prefLabel> <https://w3id.org/EnergyInformationModel/ontology/PrimaryEquipment> .
# 
# https://w3id.org/energyinformationmodel/ontology/core#a8bec9fa_deb6_4fe9_8726_0b8b6208fa73

<https://w3id.org/energyinformationmodel/ontology/core#a8bec9fa_deb6_4fe9_8726_0b8b6208fa73> a owl:Class ;
	rdfs:subClassOf <http://www.iec.ch/TC57/CIM#IdentifiedObject> ;
	rdfs:seeAlso <http://www.iec.ch/TC57/CIM#ACDCTerminal> ;
	<http://www.w3.org/2004/02/skos/core#definition> "The energy connection (the 'end') to a primary energy system function."@en ;
	<http://www.w3.org/2004/02/skos/core#editorialNote> "Generic Energy System definition of http://www.iec.ch/TC57/CIM#ACDCTerminal"@en ;
	<http://www.w3.org/2004/02/skos/core#prefLabel> "Terminal"@en .
# 
# https://w3id.org/energyinformationmodel/ontology/core#b54a2641_b1fa_46d4_8bd5_24161660e542

<https://w3id.org/energyinformationmodel/ontology/core#b54a2641_b1fa_46d4_8bd5_24161660e542> a owl:Class ;
	rdfs:subClassOf <http://www.iec.ch/TC57/CIM#IdentifiedObject> ;
	<http://www.w3.org/2004/02/skos/core#definition> "Connectivity nodes are points where terminals of primary equipment s are connected together with zero energy loss."@en ;
	<http://www.w3.org/2004/02/skos/core#editorialNote> "Generic energy system definition of http://www.iec.ch/TC57/CIM#ConnectivityNode"@en ;
	<http://www.w3.org/2004/02/skos/core#prefLabel> "ConnectivityNode"@en .
# 
# https://w3id.org/energyinformationmodel/ontology/core#c277f37c_c697_4522_9558_16d98edb8ab1

<https://w3id.org/energyinformationmodel/ontology/core#c277f37c_c697_4522_9558_16d98edb8ab1> a owl:Class ;
	rdfs:subClassOf <http://www.iec.ch/TC57/CIM#IdentifiedObject> ;
	rdfs:label "EnergieSysteemFunctie"@nl ;
	rdfs:seeAlso <http://www.iec.ch/TC57/CIM#PowerSystemResource> ;
	<http://www.w3.org/2004/02/skos/core#definition> """The Energy System Resource defines the functional elements of the energy system. The fysical stuff with which these functions are implemented are modelled by http://www.iec.ch/TC57/CIM#Asset.

An EnergySystemResource typically comes into existence during a planning/designing process and seizes to exist when either the design isn't implemented or when the part of the energy grid it models is permanently taken out of service."""@en ;
	<http://www.w3.org/2004/02/skos/core#editorialNote> "Generic energy system definition of  http://www.iec.ch/TC57/CIM#PowerSystemResource"@en ;
	<http://www.w3.org/2004/02/skos/core#prefLabel> "EnergySystemResource"@en .
# 
# Generated by the OWL API (version 4.5.9.2019-02-01T07:24:44Z) https://github.com/owlcs/owlapi
